Exercise 3.3 done

concrete-semantics/CS_Chap3.thy
@@ -119,7 +119,22 @@ lemma aval_full_asimp: "aval (full_asimp a) s = aval a s"
 
 
 (* EXERCISE 3.3 *)
+fun subst :: "vname \<Rightarrow> aexp \<Rightarrow> aexp \<Rightarrow> aexp" where
+  "subst x a (V v) = (if x = v then a else (V v))" |
+  "subst x a (N n) = (N n)" |
+  "subst x a (Plus a1 a2) = Plus (subst x a a1) (subst x a a2)"
 
+value "subst ''x'' (N 3) (Plus (V ''x'') (V ''y''))" (* It works! *)
+
+lemma substitution_lemma [simp]: "aval (subst x a e) s = aval e (s(x := aval a s))"
+  apply (induction e)
+  apply (auto)
+  done
+
+theorem "aval a1 s = aval a2 s \<Longrightarrow> aval (subst x a1 e) s = aval (subst x a2 e) s"
+  apply (induction e)
+  apply (auto)
+  done
 
 
 (* EXERCISE 3.4 *)
